2nd version

prototype/unstacked_borrows_pseudo.dfy
@@ -1,253 +1,225 @@
-datatype stack_state = Raw | Mutable | Share | Invalid | Owner
+datatype Tag = Unique(t: nat, c: nat) | SharedRO(t: nat, c:nat) | SharedRW(t: nat, c: nat) 
+              | SharedRWBot | Disabled
 
 class State {
    var counter: nat; // used to generate new id
    var mem: array<int>;
-   var tagmem: array<Pointer>;
-   var markmem: array<Pointer>; 
+   var tagmem: array<Tag>;
+   var ancestors: map<Tag, set<Tag>>;
+   var predecessor: map<Tag, Tag>;
+   // indicate if ShareRW(Bot) is on stack
+   var raw: array<bool>;   
+   // record the last SharedRO(t, c)
+   var lastread: array<Tag>;
    
-   function getStackState(addr: nat) : stack_state {
-     tagmem[addr].kind
-   }
-   
-   method generateID() returns (ret: nat) {
+   method generateID() returns (ret: nat) 
+   modifies this;
+   {
      counter := counter + 1;
      ret := counter;
    }
-   method write(p: Pointer, v: int)
-     modifies mem;
-   {
-     if (!p.valid(this)){
-       mem[p.addr] := *;
-       return;
-     }
-     
-     if (p.kind == Invalid || p.kind == Share){
-       mem[p.addr] := *;
-       return;
-     }
-     match p.kind
-     case Owner =>
-       mem[p.addr] := v;
-       tagmem[p.addr] := p;
-     case Mutable =>
-       if (p.tag == tagmem[p.addr].tag){
-          // p is the top of the stack
-          mem[p.addr] := v;
-       } else if (p.tag < tagmem[p.addr].tag){
-         // p is not on the top
-         tagmem[p.addr].kind := Invalid;  // old top is out
-         tagmem[p.addr] := p; // update the top
-         mem[p.addr] := v;
-       }
-     case Raw =>
-       if (tagmem[p.addr].tag == p.tag){
-         // p is on the top
-          mem[p.addr] := v;
-       } else{
-         mem[p.addr] := *;
-       }
+   
+   predicate isWritable(p: Pointer)
+   requires p.valid(this);
+   reads this, p;
+   { 
+      match p.tag
+      case Unique(t, c)  => p.tag in ancestors[tagmem[p.addr]]
+      case SharedRW(t, c) =>  p.tag in ancestors[tagmem[p.addr]]
+      case _ => false
    }
    
-   method read(p: Pointer) returns (r: int){
-     r := mem[p.addr];
-     if (!p.valid(this)){
-       r := *;
-       return;
-     }
-     
-     if (p.kind == Invalid){
-       r := *;
-       return;
-     }
-     match p.kind
-     case Owner =>
-       // nothing need to do
-     case Share =>
-      // nothing to do
-     case Mutable => 
-       // mutable ref
-       if (p.tag == tagmem[p.addr].tag){
-         // top
-         r := mem[p.addr];
-       } else if (p.tag < tagmem[p.addr].tag){
-         tagmem[p.addr].kind := Invalid; // old top is out
-         tagmem[p.addr] := p;
-       } 
-     }
+   method write(p: Pointer, v: int)
+     requires p.valid(this) && isWritable(p);
+     modifies mem, tagmem;
+   {
+     match p.tag
+     case Unique(t, c) =>
+       use1(p);
+       mem[p.addr] := v;
+     case SharedRW(t, c) =>
+        tagmem[p.addr] := p.tag; // update the top
+         mem[p.addr] := v;
    }
+   
+ method use1(p: Pointer) 
+ requires p.valid(this);
+{
+  match p.tag
+  case Unique(t, c) =>  
+    // Rule (USE -1 ) 
+    // requires Unique(t) is in the stack
+    // p becomes the top
+    tagmem[p.addr] := p.tag; 
+}
+
+method use2(p: Pointer)
+requires p.valid(this);
+{
+  if (raw[p.addr]) { // Pointer(l, Bot)
+    // pop up anything above SharedRWBot
+    tagmem[p.addr] := SharedRWBot;
+  } else{
+    match p.tag
+    case Unique(t, c) => // Pointer(l, t)
+    // pop up anything above Pointer(l, t)
+    tagmem[p.addr] := p.tag;
+  }
+}
+   
+   method read(p: Pointer) returns (r: int)
+   requires p.valid(this);
+   {
+     r := mem[p.addr];
+     match p.tag
+     case Unique(t, c) =>
+        use1(p);
+     case SharedRO(t, c) =>
+      // nothing to do
+     case SharedRW(t, c) => 
+      // ?
+     
+   }
+} 
    
 
 class Pointer{
   var addr: nat;
-  var tag: nat;
-  var kind: stack_state;
-  var predecessor: Pointer;
+  var tag: Tag;
   
-  predicate isAncestor(p: Pointer, s: State) 
-  requires p.valid(s);
-  {
-    (predecessor == null ==> tag == p.tag) ||
-    (predecessor != null ==> p.predecessor.tag == p.tag || predecessor.isAncestor(p, s))
+ predicate valid(s: State){
+    tag in s.ancestors[s.tagmem[addr]]
   }
   
-  predicate valid(s: State){
-    kind != Invalid &&
-    tag <= s.tagmem[addr].tag && 
-    (s.tagmem[addr].kind == kind ==> tag <= s.tagmem[addr].tag) &&
-    (s.tagmem[addr].kind != kind ==> tag == s.markmem[addr].tag)
-  }
-  
-  constructor(addr: nat, tag: nat, kind: stack_state, pred: Pointer) {
+  constructor(addr: nat, tag: Tag) {
     this.addr := addr;
     this.tag := tag;
-    this.kind := kind;
-    this.predecessor := pred;
   }
-  
 }
 
-method createOwner(addr: nat, s: State)  returns(ret: Pointer) {
+method createOwner(addr: nat, s: State)  returns(ret: Pointer) 
+modifies s;
+{
    var newID := s.generateID();
-   ret := new Pointer(addr, newID, Owner, null);
+   var new_tag := Unique(newID, 1);
+   ret := new Pointer(addr, new_tag);
+   s.ancestors := s.ancestors[new_tag := {new_tag}];
+   s.predecessor := s.predecessor[new_tag := new_tag];
+   s.raw[addr] := false;
 }
-
 
 method createMutableRef(p: Pointer, s: State) returns(ret: Pointer)
+requires p.valid(s);
+modifies s;
 {
   var newID := s.generateID();
   
-  if (!p.valid(s)) {
-    s.mem[p.addr] := *;
-    return;
-  }
-  // mutable borrowing is from mutable ref or owner
-  if (p.kind != Mutable || p.kind != Owner) {
-     s.mem[p.addr] := *;
-     return;
-  }
+  var predecessor_of_top := s.predecessor[p.tag];
+  var ancestors_of_top := s.ancestors[p.tag];
   
-  // get the state of the stack;
-  var stack_status := s.getStackState(p.addr);
-  
-  match stack_status
-  case Invalid => s.mem[p.addr] := *;
-  case Share => 
-       // pop the top
-       s.tagmem[p.addr].kind := Invalid;
-        ret := new Pointer(p.addr, newID, Mutable, s.markmem[p.addr]);
-       s.tagmem[p.addr] := ret;  // push new mut ref
-  case Mutable =>
-      // p is the top of the stack && p is mutable
-      if (s.tagmem[p.addr].tag == p.tag){
-        ret := new Pointer(p.addr, newID, Mutable, s.tagmem[p.addr]);
-        s.tagmem[p.addr] := ret;
-      } else if (s.tagmem[p.addr].isAncestor(p, s)){
-         // p is an ancestor of the top
-        var oldtop := s.tagmem[p.addr];
-        oldtop.kind := Invalid;  // old top is out
-        ret := new Pointer(p.addr, newID, Mutable, p);
-        s.tagmem[p.addr] := ret; // new top
-      } 
-    case Owner =>
-       s.markmem[p.addr] := s.tagmem[p.addr];
-       ret := new Pointer(p.addr, newID, Mutable, p);
-       s.tagmem[p.addr] := ret;
+  match p.tag
+    case Unique(t, c) =>
+        /*
+            let x = & mut p;
+            1. it is considered as a use of p
+            2. generate a fresh tag for the new reference x, i.e., Unique(t', c)
+            3. record Unique(t', c)'s predecessor
+            4. record Unique(t',c)'s ancestors
+            5. push Unique(t', c) to the stack
+        */
+       var top := s.tagmem[p.addr];
+       var newtag := Unique(newID, c);
+       s.use1(p);
+       ret := new Pointer(p.addr, newtag);
+       s.predecessor := s.predecessor[newtag := predecessor_of_top];
+       s.ancestors := s.ancestors[newtag := ancestors_of_top + {newtag}];
+       s.tagmem[p.addr] := newtag;
     case Raw =>
        // todo
 }
 
-method createShareRef(p: Pointer, s: State) returns(ret: Pointer){
+/*
+Rule (NEW-SHARE-REF-1)
+*/
+method createShareRef(p: Pointer, s: State) returns(ret: Pointer)
+requires p.valid(s);
+modifies s;
+{
   var newID := s.generateID();
-  if (!p.valid(s)) {
-    s.mem[p.addr] := *;
-    return;
-  }
+  var predecessor_of_top := s.predecessor[p.tag];
+  var ancestors_of_top := s.ancestors[p.tag];
   
-  // shared borrowing is from mutable ref or owner or shared ref
-  if (p.kind != Mutable || p.kind != Owner || p.kind != Share) {
-     s.mem[p.addr] := *;
-     return;
-  }
-  
-  // get the state of the stack;
-  var stack_status := s.getStackState(p.addr);
-  
-  match stack_status
-  case Invalid => s.mem[p.addr] := *;
-  case Share =>
-     // we consider the original mutable ref as its predecessor
-     ret := new Pointer(p.addr, newID, Share, s.markmem[p.addr]);
-     s.tagmem[p.addr] := ret; // just push
-  case Owner =>
-     // saving the owner to the marker
-     s.markmem[p.addr] := s.tagmem[p.addr]; 
-     ret := new Pointer(p.addr, newID, Share, p);
-     s.tagmem[p.addr] := ret; // push
-  case Mutable =>
-        // saving the mutable to the marker
-        s.markmem[p.addr] := s.tagmem[p.addr];
-        ret := new Pointer(p.addr, newID, Share, p);
-        s.tagmem[p.addr] := ret;
-  case Raw =>
-     // convert from raw to & mutable
-       // pop up te top
-       s.tagmem[p.addr].kind := Invalid;
-       ret := new Pointer(p.addr, newID, Mutable, s.markmem[p.addr]);
-       s.tagmem[p.addr] := ret;
+  /*
+  1. consider a read access to p
+  2. generate a fresh tag for the new reference x, i.e., SharedRO(t', c)
+  3. record SharedRO(t', c)'s predecessor
+  4. record SharedRO(t', c)'s ancestors
+  5. update lastread as SharedRO(t', c)
+  6. push SharedRO(t', c) to the stack
+  */
+  readPointer(p, s);
+  var newtag := SharedRO(newID, 1);
+  ret := new Pointer(p.addr, newtag);
+  s.predecessor := s.predecessor[newtag := predecessor_of_top];
+  s.ancestors := s.ancestors[newtag := ancestors_of_top + {newtag}];
+  s.lastread[p.addr] := newtag;
+  s.tagmem[p.addr] := newtag;
 }
 
-method createRawRef(p: Pointer, s: State) returns(ret: Pointer)
-modifies s.mem;
+// Rule READ-1
+// p could be Unique(t, c), SharedRO(t, c), SharedRW(t, c)
+method readPointer(p: Pointer, s: State)
+requires p.valid(s) ;
+modifies s, s.tagmem;
 {
-   var newID := s.generateID();
-   if (!p.valid(s)) {
-    s.mem[p.addr] := *;
-    return;
-  }
-   
-   // raw borrowing is from mutable ref or owner
-  if (p.kind != Mutable || p.kind != Owner) {
-     s.mem[p.addr] := *;
-     return;
-  }
+  // pop items off the stack until all the items above the item 
+  // with tag t are SharedRO(t, c)
+  s.tagmem[p.addr] := s.lastread[p.addr];
+}
+
+/*
+Raw pointers can only be created from Unique(t)
+let raw_pointer = &mut p as *mut i32;
+*/
+method createMutableRawRef(p: Pointer, s: State) returns(ret: Pointer)
+requires p.valid(s);
+modifies s;
+{
+  var newID := s.generateID();
+  var top := s.tagmem[p.addr];
+  var predecessor_of_top := s.predecessor[p.tag];
+  var ancestors_of_top := s.ancestors[p.tag];
   
-  // get the state of the stack;
-  var stack_status := s.getStackState(p.addr);
-  
-  match stack_status
-  case Mutable =>
-    if (p.tag == s.tagmem[p.addr].tag){
-      // p is on the top
-      // saving top to the marker
-      s.markmem[p.addr] := s.tagmem[p.addr];
-      ret := new Pointer(p.addr, newID, Raw, s.markmem[p.addr]);
-      s.tagmem[p.addr] := ret;
-    } else if (p.tag < s.tagmem[p.addr].tag){
-      // saving p to the marker
-      s.markmem[p.addr] := p;
-      // old top is out
-      s.tagmem[p.addr].kind := Invalid;
-      ret := new Pointer(p.addr, newID, Raw, s.markmem[p.addr]);
-      s.tagmem[p.addr] := ret;
-    }
-   case Owner =>
-     if (p.tag != s.tagmem[p.addr].tag){
-      s.mem[p.addr] := *;
-     } else{
-       // saving owner to the marker
-       s.markmem[p.addr] := s.tagmem[p.addr];
-       ret := new Pointer(p.addr, newID, Raw, s.markmem[p.addr]);
-       s.tagmem[p.addr] := ret;
-     }
-   case Raw =>
-     // top is out
-     s.tagmem[p.addr].kind := Invalid;
-     // we only know the ref from marker,
-     // which was the top mutable or owner before the first raw sharing
-     if (p.tag == s.markmem[p.addr].tag){
-       ret := new Pointer(p.addr, newID, Raw, s.markmem[p.addr]);
-       s.tagmem[p.addr] := ret;
-     } 
-  
+  match p.tag
+  case ShareRWBot =>
+      /*
+      1. a use of p
+      2. generate new pointer
+      3. record new tag's predecessor
+      4. record new tag's ancestors
+      5. push ShareRW(BOT) on the top
+      */
+      var newtag := Unique(newID, 1);
+      s.use2(p);
+      var ret := new Pointer(p.addr, newtag);
+      s.predecessor := s.predecessor[newtag := top];
+      s.ancestors := s.ancestors[newtag := s.ancestors[top] + {newtag}];
+      s.tagmem[p.addr] := newtag;
+   case Unique(t, c) =>
+      /*
+      Rule (NEW-MUTABLE-RAW-1)
+      1. a use of p (USE-2)
+      2. generate new pointer
+      3. record new tag's predecessor
+      4. record new tag's ancestors
+      5. push ShareRW(BOT) on the top
+      6. mark the addr as raw
+      */
+      var newtag := SharedRWBot;
+      s.use2(p);
+      var ret := new Pointer(p.addr, newtag);
+      s.predecessor := s.predecessor[newtag := predecessor_of_top];
+      s.ancestors := s.ancestors[newtag := ancestors_of_top + {newtag}];
+      s.tagmem[p.addr] := newtag;
+      s.raw[p.addr] := true;
 }
